Weidenbach_Book/IsaSAT/IsaSAT_Restart_Simp_LLVM.thy
@@ -3,7 +3,7 @@ imports  IsaSAT_Restart_Heuristics_LLVM IsaSAT_Garbage_Collect_LLVM
   IsaSAT_Other_LLVM IsaSAT_Propagate_Conflict_LLVM IsaSAT_Inprocessing_LLVM IsaSAT_Restart_LLVM
 begin
 
-sepref_register cdcl_twl_full_restart_wl_prog_heur mark_to_delete_clauses_GC_wl_D_heur
+sepref_register cdcl_twl_mark_clauses_to_delete mark_to_delete_clauses_GC_wl_D_heur
 
 sepref_def cdcl_twl_restart_wl_heur_fast_code
   is \<open>cdcl_twl_restart_wl_heur\<close>
@@ -12,10 +12,10 @@ sepref_def cdcl_twl_restart_wl_heur_fast_code
   supply [[goals_limit = 1]]
   by sepref
 
-sepref_def cdcl_twl_full_restart_wl_prog_heur_fast_code
-  is \<open>cdcl_twl_full_restart_wl_prog_heur\<close>
+sepref_def cdcl_twl_mark_clauses_to_delete_fast_code
+  is \<open>cdcl_twl_mark_clauses_to_delete\<close>
   :: \<open>[\<lambda>S. length (get_clauses_wl_heur S) \<le> sint64_max]\<^sub>a isasat_bounded_assn\<^sup>d \<rightarrow> isasat_bounded_assn\<close>
-  unfolding cdcl_twl_full_restart_wl_prog_heur_def
+  unfolding cdcl_twl_mark_clauses_to_delete_def
   supply [[goals_limit = 1]]
   by sepref
 
@@ -97,7 +97,7 @@ begin
     restart_required_heur_fast_code
     cdcl_twl_full_restart_wl_D_GC_heur_prog_fast_code
     cdcl_twl_restart_wl_heur_fast_code
-    cdcl_twl_full_restart_wl_prog_heur_fast_code
+    cdcl_twl_mark_clauses_to_delete_fast_code
     cdcl_twl_local_restart_wl_D_heur_fast_code
    get_conflict_wl_is_None_fast_code
 end
